src/CSL/Adequacy.v
@@ -283,3 +283,58 @@ Proof.
   iDestruct ("Hφ" with "Hσ") as (E) ">Hφ".
   iMod (fupd_intro_mask') as "_"; last by iModIntro. solve_ndisj.
 Qed.
+
+Import RelationNotations.
+
+Theorem wp_recovery_invariance {T R} OpT Σ Λ `{invPreG Σ} s (e: proc OpT T) (rec: proc OpT R)
+        σ1 σ2 t2 (φ ρ : Λ.(State) → Prop) :
+  (* φ is an invariant of normal execution *)
+  (∀ `{Hinv : invG Σ},
+     (|={⊤}=> ∃ stateI : State Λ → iProp Σ,
+       let _ : irisG OpT Λ Σ := IrisG _ _ _ Hinv stateI in
+       stateI σ1 ∗ WP e @ s; ⊤ {{ _, True }} ∗ (∀ σ2', stateI σ2' ={⊤,∅}=∗ ⌜φ σ2'⌝))%I) →
+  (* φ is an invariant of recovery execution *)
+  (∀ `{Hinv : invG Σ} σ1 σ1' (Hφ: φ σ1) (Hcrash: Λ.(crash_step) σ1 σ1' tt),
+     (|={⊤}=> ∃ stateI : State Λ → iProp Σ,
+       let _ : irisG OpT Λ Σ := IrisG _ _ _ Hinv stateI in
+       stateI σ1' ∗ WP rec @ s; ⊤ {{ _, True }} ∗ (∀ σ2', stateI σ2' ={⊤,∅}=∗ ⌜φ σ2'⌝))%I) →
+  (∀ σ, φ σ → ρ σ) →
+  (∀ σ1 σ2, φ σ1 → Λ.(crash_step) σ1 σ2 tt → ρ σ2) →
+  Λ.(rexec_partial) e (rec_singleton rec) σ1 σ2 t2 →
+  ρ σ2.
+Proof.
+  intros Hwp_e Hwp_rec Himpl Hcrash_impl Hpartial.
+  unfold rexec_partial, exec_recover_partial in Hpartial.
+  destruct Hpartial as (tp&σhalt&Hpartial&Hrec).
+  (* Show that φ is preserved after halt of e *)
+  assert (Hφ: φ σhalt).
+  { eapply wp_invariance; eauto.
+    intros Hinv.
+    iMod Hwp_e as (stateI) "[Hσ [H Hφ]]". iExists stateI. iIntros "{$Hσ} {$H} !> Hσ".
+      by iApply "Hφ".
+  }
+  clear Hpartial Hwp_e.
+  eapply rimpl_elim in Hrec; last first.
+  { setoid_rewrite exec_seq_partial_singleton.
+    setoid_rewrite seq_sliding.
+    setoid_rewrite <-bind_assoc at 1.
+    reflexivity. }
+  destruct Hrec as ([]&σhalt_rec&Hhd&Hrest).
+  (* Show that φ is preserved after crash + halt of rec *)
+  assert (Hφ_halt: ∀ σhalt σhalt_rec,
+             φ σhalt ->
+             (_ <- Λ.(crash_step); exec_halt Λ rec) σhalt σhalt_rec () ->
+             φ σhalt_rec).
+  {
+    intros ??? ([]&σcrash&Hcrash&Hhalt).
+    destruct Hhalt as (tp'&?&Hpartial&[]); subst.
+    eapply wp_invariance; eauto.
+    intros Hinv.
+    iMod Hwp_rec as (stateI) "[Hσ [H Hφ]]"; eauto. iExists stateI. iIntros "{$Hσ} {$H} !> Hσ".
+      by iApply "Hφ".
+  }
+  assert (Hrec: φ σhalt_rec) by eauto.
+  clear Hwp_rec. clear Hhd.
+  revert σhalt Hrec Hφ.
+  induction Hrest as [σhalt_rec []| x y z [] []]; eauto.
+Qed.
